Linear STLC: Preserve order of vars from beta redex

stlc_linear/Stlc.v
@@ -1,5 +1,6 @@
 Require Export Coq.Unicode.Utf8.
 Require Import Coq.Program.Equality.
+Require Import Coq.Program.Tactics.
 
 (* Types
    Meta-variables: a, b
@@ -31,6 +32,15 @@ where "Γ₁ ▻▻ Γ₂" := (ecat Γ₁ Γ₂).
 
 Lemma ecat_left_empty Δ : ε ▻▻ Δ = Δ.
 Proof. induction Δ; simpl; congruence. Qed.
+
+Lemma ecat_empty_left {Γ₁ Γ₂} :
+  ε = Γ₁ ▻▻ Γ₂ → Γ₁ = ε.
+Proof. induction Γ₂; inversion 1; auto. Qed.
+
+Lemma ecat_empty_right {Γ₁ Γ₂} :
+  ε = Γ₁ ▻▻ Γ₂ → Γ₂ = ε.
+Proof. induction Γ₂; inversion 1; auto. Qed.
+
 
 (* Domains represent a set of variables such as the variables
    bound in a typing environment or that can appear in a term.
@@ -71,6 +81,20 @@ where "⟨ i ∈ γ ⟩" := (inDom γ i).
 Lemma inDomInvS (γ: Dom) (i: Ix) : ⟨S i ∈ S γ⟩ → ⟨i ∈ γ⟩.
 Proof. inversion 1; auto. Qed.
 
+(* Type environment lookup. *)
+Reserved Notation "⟪  i : a ∈ Γ  ⟫"
+  (at level 0, i at level 10, Γ at level 10).
+Inductive inEnv : Env → Ix → Ty → Prop :=
+  | inEnvO {Γ a} :
+      ⟪   O : a ∈ Γ ▻ a  ⟫
+  | inEnvS {Γ a a' i} :
+      ⟪   i : a ∈ Γ      ⟫ →
+      ⟪ S i : a ∈ Γ ▻ a' ⟫
+where "⟪  i : a ∈ Γ  ⟫" := (inEnv Γ i a).
+
+Lemma inEnvInvS (Γ: Env) (i: Ix) (a b: Ty) :
+  ⟪S i : a ∈ Γ ▻ b⟫ → ⟪ i : a ∈ Γ ⟫.
+Proof. inversion 1; auto. Qed.
 
 (* A partition of a context g is a pair of contexts (g1,g2) such that g is some
  * permutation of g1++g2, under the side condition that the domains of g1 and g2
@@ -93,6 +117,19 @@ Inductive PartDom : Part → Dom → Dom → Dom → Prop :=
       ⟨p         ⊢  γ    =  γ₁   ∘ γ₂  ⟩ →
       ⟨pright p  ⊢  S γ  =  γ₁   ∘ S γ₂⟩
 where "⟨ p ⊢ γ = γ₁ ∘ γ₂ ⟩" := (PartDom p γ γ₁ γ₂).
+
+(* Partition typing environments. *)
+Reserved Notation "⟪ p ⊢ Γ = Γ₁ ∘ Γ₂ ⟫"
+  (at level 0, p at level 10, Γ at level 10, Γ₁ at level 10, Γ₂ at level 10).
+Inductive PartEnv : Part → Env → Env → Env → Prop :=
+  | PENil : ⟪ pnil ⊢ ε = ε ∘ ε ⟫
+  | PELeft {p a Γ Γ₁ Γ₂} :
+      ⟪ p         ⊢  Γ       =  Γ₁       ∘ Γ₂       ⟫ →
+      ⟪ pleft p   ⊢  (Γ ▻ a) =  (Γ₁ ▻ a) ∘ Γ₂       ⟫
+  | PERight {p a Γ Γ₁ Γ₂} :
+      ⟪ p         ⊢  Γ       =  Γ₁       ∘ Γ₂       ⟫ →
+      ⟪ pright p  ⊢  (Γ ▻ a) =  Γ₁       ∘ (Γ₂ ▻ a) ⟫
+where "⟪ p ⊢ Γ = Γ₁ ∘ Γ₂ ⟫" := (PartEnv p Γ Γ₁ Γ₂).
 
 (* Given a partition γ = γ₁ ∘ γ₂ map variables from γ₁ to γ. *)
 Fixpoint fromLeft (p: Part) (i : Ix) : Ix :=
@@ -142,6 +179,32 @@ Proof with simpl; eauto using inDom, inDomInvS.
   induction pd... destruct i...
 Qed.
 
+
+Lemma fromLeft_inEnv {p Γ Γ₁ Γ₂} (pe: ⟪ p ⊢ Γ = Γ₁ ∘ Γ₂⟫) :
+  ∀ (i: Ix) a, ⟪i : a ∈ Γ₁⟫ → ⟪fromLeft p i : a ∈ Γ⟫.
+Proof with simpl; eauto using inEnv, inEnvInvS.
+  induction pe... destruct i... inversion 1...
+Qed.
+
+Lemma fromRight_inEnv {p Γ Γ₁ Γ₂} (pe: ⟪p ⊢ Γ = Γ₁ ∘ Γ₂⟫) :
+  ∀ (i: Ix) a, ⟪i : a ∈ Γ₂⟫ → ⟪fromRight p i :a ∈ Γ⟫.
+Proof with simpl; eauto using inEnv, inEnvInvS.
+  induction pe... destruct i... inversion 1...
+Qed.
+
+Lemma fromLeft_inEnvInv {p Γ Γ₁ Γ₂} (pe: ⟪p ⊢ Γ = Γ₁ ∘ Γ₂⟫) :
+  ∀ (i: Ix) a, ⟪fromLeft p i : a ∈ Γ⟫ → ⟪i : a ∈ Γ₁⟫.
+Proof with simpl; eauto using inEnv, inEnvInvS.
+  induction pe... destruct i... inversion 1...
+Qed.
+
+Lemma fromRight_inEnvInv {p Γ Γ₁ Γ₂} (pe: ⟪p ⊢ Γ = Γ₁ ∘ Γ₂⟫) :
+  ∀ (i: Ix) a, ⟪fromRight p i : a ∈ Γ⟫ → ⟪i : a ∈ Γ₂⟫.
+Proof with simpl; eauto using inEnv, inEnvInvS.
+  induction pe... destruct i... inversion 1...
+Qed.
+
+
 (* Given a partition γ = γ₁ ∘ γ₂, decide for a variable in
    γ if it is in γ₁ or γ₂ and return an approporiate index. *)
 Fixpoint isLeftOrRight (p: Part) (i: Ix) : Ix + Ix :=
@@ -163,25 +226,63 @@ Fixpoint isLeftOrRight (p: Part) (i: Ix) : Ix + Ix :=
                   end
   end.
 
+Lemma partLeftEmpty {pΓΔ ΓΔ Δ} (peΓΔ: ⟪ pΓΔ ⊢ ΓΔ = ε ∘ Δ ⟫) : ΓΔ = Δ.
+Proof. depind peΓΔ; simpl; congruence. Qed.
+
+Ltac crush' :=
+  intros; simpl in *;
+  repeat
+    (try match goal with
+           | [ H: inl _ = inl _ |- _ ] => inversion H; clear H; subst
+           | [ H: inr _ = inr _ |- _ ] => inversion H; clear H; subst
+           | [ H: match ?i with _ => _ end = inl _ |- _ ] =>
+             destruct i eqn: ?
+           | [ H: match ?i with _ => _ end = inr _ |- _ ] =>
+             destruct i eqn: ?
+         end;
+     subst;
+     try discriminate;
+     eauto).
+
+Lemma isLeftOrRight_inl p :
+  ∀ i j, isLeftOrRight p i = inl j → i = fromLeft p j.
+Proof. induction p; crush'.
+Qed.
+
+Lemma isLeftOrRight_inr p :
+  ∀ i j, isLeftOrRight p i = inr j → i = fromRight p j.
+Proof. induction p; crush'. Qed.
+
 Ltac crush :=
   intros;
   repeat
-    (repeat
+    (try
        match goal with
+         | [ H: ?x = ?x |- _ ] => clear H
+         | [ H: ?x ≠ ?x |- _ ] => destruct H
+
+         (* Naturals (Domains, Indices) *)
          | [ H: S _ = S _     |- _ ] => apply eq_add_S in H
+         | [ |- S _ = S _ ] => f_equal
+
+         (* Coproducts *)
          | [ H: inl _ = inl _ |- _ ] => inversion H; clear H; subst
          | [ H: inr _ = inr _ |- _ ] => inversion H; clear H; subst
          | [ H: inl _ = inr _ |- _ ] => inversion H
          | [ H: inr _ = inl _ |- _ ] => inversion H
-         | [ H: ⟨_   ∈ O⟩     |- _ ] => inversion H
-         | [ H: ⟨O   ∈ S _⟩   |- _ ] => clear H
-         | [ H: ⟨S _ ∈ S _⟩   |- _ ] => apply inDomInvS in H
-         | [ H: ⟨?i  ∈ S _⟩   |- context[match ?i with _ => _ end] ] =>
-           destruct i
-         | [ H: ⟨?i  ∈ S _⟩, H1: context[match ?i with _ => _ end] |- _ ] =>
-           destruct i
-         | [ |- S _ = S _ ] => f_equal
-         | [ |- ⟨S _ ∈ S _⟩ ] => constructor
+         | [ |- inl _ = inl _ ] => f_equal
+         | [ |- inr _ = inr _ ] => f_equal
+
+         (* Environments *)
+         | [ H : _ ▻ _ = _ ▻ _ |- _ ] =>
+           inversion H; clear H
+         | [ H : [_] = _ ▻ _ |- _ ] =>
+           unfold singleton in H; inversion H; clear H
+         | [ H : _ ▻ _ = [_] |- _ ] =>
+           unfold singleton in H; inversion H; clear H
+         | [ |- _ ▻ _ = _ ▻ _ ] => f_equal
+
+         (* Partitioning *)
          | [ H: match ?i with _ => _ end = inl _ |- _ ] =>
            destruct i eqn: ?
          | [ H: match ?i with _ => _ end = inr _ |- _ ] =>
@@ -190,24 +291,78 @@ Ltac crush :=
            destruct (isLeftOrRight p i) eqn: ?
          | [ |- context[match isLeftOrRight ?p ?i with _ => _ end] ] =>
            destruct (isLeftOrRight p i) eqn: ?
+         | [ |- pleft _ = pleft _ ] => f_equal
+         | [ |- pright _ = pright _ ] => f_equal
+         | [ H: isLeftOrRight _ ?i = inl _, wi: ⟪ ?i : _ ∈ _ ⟫ |- _ ] =>
+           apply isLeftOrRight_inl in H
+         | [ H: isLeftOrRight _ ?i = inr _, wi: ⟪ ?i : _ ∈ _ ⟫ |- _ ] =>
+           apply isLeftOrRight_inr in H
+         (* | [ H: context[fromLeft (pright ?p) ?i] |- _ ] => *)
+         (*   change (fromLeft (pright p) i) with (S (fromLeft p i)) in H *)
+         (* | [ H: context[fromRight (pleft ?p) ?i] |- _ ] => *)
+         (*   change (fromRight (pleft p) i) with (S (fromRight p i)) in H *)
+
+         (* Dom containment *)
+         | [ H: ⟨_   ∈ O⟩     |- _ ] => inversion H
+         | [ H: ⟨O   ∈ S _⟩   |- _ ] => clear H
+         | [ H: ⟨S _ ∈ S _⟩   |- _ ] => apply inDomInvS in H
+         | [ H: ⟨?i  ∈ S _⟩   |- context[match ?i with _ => _ end] ] =>
+           destruct i
+         | [ H: ⟨?i  ∈ S _⟩, H1: context[match ?i with _ => _ end] |- _ ] =>
+           destruct i
+         | [ |- ⟨S _ ∈ S _⟩ ] => constructor
+         | [ H: ⟨ match ?i with _ => _ end ∈ S _ ⟩ |- _ ] =>
+           destruct i eqn: ?
+         | [ H: ⟨fromLeft (pleft _) ?i ∈ S _⟩ |- _ ] =>
+           destruct i eqn: ?
+         | [ H: ⟨fromRight (pright _) ?i ∈ S _⟩ |- _ ] =>
+           destruct i eqn: ?
+
+         (* Env containment *)
+         | [ H: ⟪_   : _ ∈ ε    ⟫ |- _ ] => inversion H
+         | [ H: ⟪O   : _ ∈ _ ▻ _⟫ |- _ ] => inversion H; clear H
+         | [ H: ⟪S _ : _ ∈ _ ▻ _⟫ |- _ ] => apply inEnvInvS in H
+         | [ H: ⟪?i  : _ ∈ _ ▻ _⟫ |- context[match ?i with _ => _ end] ] =>
+           destruct i
+         | [ H: ⟪?i  : _ ∈ _ ▻ _⟫, H1: context[match ?i with _ => _ end] |- _ ] =>
+           destruct i
+         | [ |- ⟪S _ : _ ∈ _ ▻ _⟫ ] => econstructor
+         | [ |- ⟪ 0 : ?a ∈ (_ ▻ ?a) ⟫ ] => constructor
+         | [ H: ⟪_   : _ ∈ [_] ⟫ |- _ ] => inversion H; clear H
+         | [ H: ⟪ match ?i with _ => _ end : _ ∈ _ ▻ _ ⟫ |- _ ] =>
+           destruct i eqn: ?
+         | [ H: ⟪fromLeft (pleft _) ?i : _ ∈ _ ▻ _⟫ |- _ ] =>
+           destruct i eqn: ?
+         | [ H: ⟪fromRight (pright _) ?i : _ ∈ _ ▻ _⟫ |- _ ] =>
+           destruct i eqn: ?
+
+         (* Dom partitioning *)
          | [ pd: ⟨?p ⊢ ?γ = _ ∘ _⟩, wi: ⟨ fromLeft ?p _ ∈ ?γ ⟩ |- _ ] =>
            apply (fromLeft_inDomInv pd) in wi
          | [ pd: ⟨?p ⊢ ?γ = _ ∘ _⟩, wi: ⟨ fromRight ?p _ ∈ ?γ ⟩ |- _ ] =>
            apply (fromRight_inDomInv pd) in wi
+
+         (* Env partitioning *)
+         | [ pe: ⟪ _        ⊢ _       = ε ∘ _ ⟫ |- _ ] => apply partLeftEmpty in pe
+         | [ pe: ⟪ _        ⊢ ε       = _ ∘ _ ⟫ |- _ ] => inversion pe; clear pe
+         | [ pe: ⟪ pnil     ⊢ _       = _ ∘ _ ⟫ |- _ ] => inversion pe; clear pe
+         | [ pe: ⟪ _        ⊢ (_ ▻ _) = _ ∘ _ ⟫ |- _ ] => inversion pe; clear pe
+         | [ pe: ⟪ pleft _  ⊢ _       = _ ∘ _ ⟫ |- _ ] => inversion pe; clear pe
+         | [ pe: ⟪ pright _ ⊢ _       = _ ∘ _ ⟫ |- _ ] => inversion pe; clear pe
+         | [ pe: ⟪?p ⊢ ?Γ = _ ∘ _⟫, wi: ⟪ fromLeft ?p _ : _ ∈ ?γ ⟫ |- _ ] =>
+           apply (fromLeft_inEnvInv pe) in wi
+         | [ pe: ⟪?p ⊢ ?Γ = _ ∘ _⟫, wi: ⟪ fromRight ?p _ : _ ∈ ?γ ⟫ |- _ ] =>
+           apply (fromRight_inEnvInv pe) in wi
+
+         | [ |- ⟪ pleft _  ⊢ _       = _ ∘ _ ⟫ ] => econstructor
+         | [ |- ⟪ pright _ ⊢ _       = _ ∘ _ ⟫ ] => econstructor
+
        end;
      simpl in *;
      subst;
      try discriminate;
      try rewrite dunion_left_zero in *;
      eauto using inDom).
-
-Lemma isLeftOrRight_inl_sound p :
-  ∀ i j, isLeftOrRight p i = inl j → i = fromLeft p j.
-Proof. induction p; crush. Qed.
-
-Lemma isLeftOrRight_inr_sound p :
-  ∀ i j, isLeftOrRight p i = inr j → i = fromRight p j.
-Proof. induction p; crush. Qed.
 
 Lemma isLeftOrRight_inl_inDom {p γ γ₁ γ₂} (pd: ⟨p ⊢ γ = γ₁ ∘ γ₂⟩) :
   ∀ {i j}, ⟨i ∈ γ⟩ → isLeftOrRight p i = inl j → ⟨j ∈ γ₁⟩.
@@ -217,99 +372,16 @@ Lemma isLeftOrRight_inr_inDom {p γ γ₁ γ₂} (pd: ⟨p ⊢ γ = γ₁ ∘ γ
   ∀ {i j}, ⟨i ∈ γ⟩ → isLeftOrRight p i = inr j → ⟨j ∈ γ₂⟩.
 Proof. induction pd; crush. Qed.
 
-(* Replace a single binding for i by δ bindings. *)
-Fixpoint insertDom (δ: Dom) (γ: Dom) (i: Ix) : Dom :=
-  match γ , i with
-    | O   , _   => O
-    | S γ , O   => γ ∪ δ
-    | S γ , S i => S (insertDom δ γ i)
-  end.
-
-Lemma insertDom_foo δ γ₁ γ₂ :
-  insertDom δ (γ₁ ∪ 1 ∪ γ₂) γ₂ = γ₁ ∪ δ ∪ γ₂.
-Proof. induction γ₂; crush. Qed.
-
-Fixpoint plefts (p: Part) (δ: Dom) : Part :=
-  match δ with
-    | O   => p
-    | S δ => pleft (plefts p δ)
-  end.
-
-Fixpoint prights (p: Part) (δ: Dom) : Part :=
-  match δ with
-    | O   => p
-    | S δ => pright (prights p δ)
-  end.
-
-Lemma plefts_partdom δ {p γ γ₁ γ₂} (pd: ⟨p ⊢ γ = γ₁ ∘ γ₂⟩) :
-  ⟨plefts p δ ⊢ (γ ∪ δ) = (γ₁ ∪ δ) ∘ γ₂⟩.
-Proof. induction δ; simpl; eauto using PartDom. Qed.
-
-Lemma prights_partdom δ {p γ γ₁ γ₂} (pd: ⟨p ⊢ γ = γ₁ ∘ γ₂⟩) :
-  ⟨prights p δ ⊢ (γ ∪ δ) = γ₁ ∘ (γ₂ ∪ δ)⟩.
-Proof. induction δ; simpl; eauto using PartDom. Qed.
-
-(* Partition typing environments. *)
-Reserved Notation "⟪ p ⊢ Γ = Γ₁ ∘ Γ₂ ⟫"
-  (at level 0, p at level 10, Γ at level 10, Γ₁ at level 10, Γ₂ at level 10).
-Inductive PartEnv : Part → Env → Env → Env → Prop :=
-  | PENil : ⟪ pnil ⊢ ε = ε ∘ ε ⟫
-  | PELeft {p a Γ Γ₁ Γ₂} :
-      ⟪ p         ⊢  Γ       =  Γ₁       ∘ Γ₂       ⟫ →
-      ⟪ pleft p   ⊢  (Γ ▻ a) =  (Γ₁ ▻ a) ∘ Γ₂       ⟫
-  | PERight {p a Γ Γ₁ Γ₂} :
-      ⟪ p         ⊢  Γ       =  Γ₁       ∘ Γ₂       ⟫ →
-      ⟪ pright p  ⊢  (Γ ▻ a) =  Γ₁       ∘ (Γ₂ ▻ a) ⟫
-where "⟪ p ⊢ Γ = Γ₁ ∘ Γ₂ ⟫" := (PartEnv p Γ Γ₁ Γ₂).
-
-Lemma plefts_partenv Δ {p Γ Γ₁ Γ₂} (pe: ⟪ p ⊢ Γ = Γ₁ ∘ Γ₂ ⟫) :
-  ⟪ plefts p (dom Δ) ⊢ (Γ ▻▻ Δ) = (Γ₁ ▻▻ Δ) ∘ Γ₂ ⟫.
-Proof. induction Δ; simpl; eauto using PartEnv. Qed.
-
-Lemma prights_partenv Δ {p Γ Γ₁ Γ₂} (pe: ⟪ p ⊢ Γ = Γ₁ ∘ Γ₂ ⟫) :
-  ⟪ prights p (dom Δ) ⊢ (Γ ▻▻ Δ) = Γ₁ ∘ (Γ₂ ▻▻ Δ) ⟫.
-Proof. induction Δ; simpl; eauto using PartEnv. Qed.
-
-Hint Constructors PartDom.
-Hint Resolve plefts_partdom.
-Hint Resolve prights_partdom.
-
-Hint Constructors PartEnv.
-Hint Resolve plefts_partenv.
-Hint Resolve prights_partenv.
-
-(* Type environment lookup. *)
-Reserved Notation "⟪  i : a ∈ Γ  ⟫"
-  (at level 0, i at level 10, Γ at level 10).
-Inductive wtIx : Env → Ix → Ty → Prop :=
-  | wt0 {Γ a} :
-      ⟪   O : a ∈ Γ ▻ a  ⟫
-  | wtS {Γ a a' i} :
-      ⟪   i : a ∈ Γ      ⟫ →
-      ⟪ S i : a ∈ Γ ▻ a' ⟫
-where "⟪  i : a ∈ Γ  ⟫" := (wtIx Γ i a).
-
 Lemma wtix_isLeftOrRight_inl {p Γ Γ₁ Γ₂} (pe: ⟪ p ⊢ Γ = Γ₁ ∘ Γ₂ ⟫) :
   ∀ {a i j}, ⟪ i : a ∈ Γ ⟫ → isLeftOrRight p i = inl j → ⟪ j : a ∈ Γ₁ ⟫.
-Proof with crush.
-  induction pe...
-  - inversion H...
-    constructor...
-  - inversion H...
-    constructor...
-  - inversion H...
-Qed.
+Proof. induction pe; crush. Qed.
 
 Lemma wtix_isLeftOrRight_inr {p Γ Γ₁ Γ₂} (pe: ⟪ p ⊢ Γ = Γ₁ ∘ Γ₂ ⟫) :
   ∀ {a i j}, ⟪ i : a ∈ Γ ⟫ → isLeftOrRight p i = inr j → ⟪ j : a ∈ Γ₂ ⟫.
-Proof with crush.
-  induction pe...
-  - inversion H...
-  - inversion H...
-    constructor...
-  - inversion H...
-    constructor...
-Qed.
+Proof. induction pe; crush. Qed.
+
+Hint Constructors PartDom.
+Hint Constructors PartEnv.
 
 (* Terms.
    Meta-variables: s, t
@@ -350,108 +422,243 @@ Inductive wtTm : Env → Tm → Ty → Prop :=
       ⟪ Γ ⊢ app p t₁ t₂ : b ⟫
 where "⟪  Γ ⊢ t : T  ⟫" := (wtTm Γ t T).
 
-(* Updates the partition witness when substituting index i for
-   a term with δ free variables. *)
-Fixpoint substPart (p: Part) (i: Ix) (δ: Dom): Part :=
-  match p with
-    | pnil    => pnil
-    | pleft p =>
-      match i with
-        | O   => plefts p δ
-        | S i => pleft (substPart p i δ)
-      end
-    | pright p =>
-      match i with
-        | O   => prights p δ
-        | S i => pright (substPart p i δ)
-      end
+(* The substitution function
+     substTm (i: Ix) (p: Part) (s t: Tm) : Tm
+   takes as inputs
+     i: The index to be substituted.
+     s: The term that substitutes the index.
+     t: The term in which the substitution is performed.
+     p: A partitioning witness that determines the final
+        order of the indices.
+
+   Assume Δ ⊢ s, Γ ⊢ t, i ∈ Γ and p ⊢ ΓΔ = Γ ∘ Δ. Then the final context will be
+   ΓΔ with the index i removed (substResultEnv ΓΔ pΓΔ i). We call ΓΔ the input
+   environment (which is not given at the term level) and p the input
+   partition. At each split point with partition p' we have to decide whether to
+   proceed left or right with the substitution. The following functions
+   calculuate the input environment and partition and also the new result
+   partition for the split point that replaces p'.
+ *)
+
+Fixpoint substLeftInputEnv (ΓΔ: Env) (pΓΔ pΓ: Part) : Env :=
+  match ΓΔ , pΓΔ , pΓ with
+    | ε      , _          , _         => ε
+    | _      , pnil       , _         => ε
+    | ΓΔ ▻ a , pleft pΓΔ  , pnil      => ε
+    | ΓΔ ▻ a , pleft pΓΔ  , pleft pΓ  => substLeftInputEnv ΓΔ pΓΔ pΓ ▻ a
+    | ΓΔ ▻ a , pleft pΓΔ  , pright pΓ => substLeftInputEnv ΓΔ pΓΔ pΓ
+    | ΓΔ ▻ a , pright pΓΔ , pΓ        => substLeftInputEnv ΓΔ pΓΔ pΓ ▻ a
   end.
 
-Lemma substPart_inl_partdom {p γ γ₁ γ₂} (pd: ⟨p ⊢ γ = γ₁ ∘ γ₂⟩) :
-  ∀ i j δ,
-    isLeftOrRight p i = inl j →
-    ⟨substPart p i δ ⊢ insertDom δ γ i = insertDom δ γ₁ j ∘ γ₂⟩.
-Proof. induction pd; crush. Qed.
-
-Lemma substPart_inr_partdom {p γ γ₁ γ₂} (pd: ⟨p ⊢ γ = γ₁ ∘ γ₂⟩) :
-  ∀ i j δ,
-    isLeftOrRight p i = inr j →
-    ⟨substPart p i δ ⊢ insertDom δ γ i = γ₁ ∘ insertDom δ γ₂ j⟩.
-Proof. induction pd; crush. Qed.
-
-Fixpoint insertEnv (Δ: Env) (Γ: Env) (i: Ix) : Env :=
-  match Γ , i with
-    | ε     , _   => ε
-    | Γ ▻ a , O   => Γ ▻▻ Δ
-    | Γ ▻ a , S i => insertEnv Δ Γ i ▻ a
+Fixpoint substLeftInputPart (pΓΔ pΓ: Part) : Part :=
+  match pΓΔ , pΓ with
+    | pnil       , _         => pnil
+    | pleft _    , pnil      => pnil
+    | pleft pΓΔ  , pleft pΓ  => pleft (substLeftInputPart pΓΔ pΓ)
+    | pleft pΓΔ  , pright pΓ => substLeftInputPart pΓΔ pΓ
+    | pright pΓΔ , pΓ        => pright (substLeftInputPart pΓΔ pΓ)
   end.
 
-Lemma insertEnv_foo a Δ Γ₁ Γ₂ :
-  insertEnv Δ (Γ₁ ▻▻ [a] ▻▻ Γ₂) (dom Γ₂) = Γ₁ ▻▻ Δ ▻▻ Γ₂.
-Proof. induction Γ₂; simpl in *; congruence. Qed.
+Lemma substLeftInput {pΓΔ ΓΔ Γ Δ} (peΓΔ : ⟪ pΓΔ ⊢ ΓΔ = Γ ∘ Δ ⟫) :
+  ∀ {pΓ Γ₁ Γ₂},
+    ⟪ pΓ ⊢ Γ = Γ₁ ∘ Γ₂ ⟫ →
+    ⟪ substLeftInputPart pΓΔ pΓ
+      ⊢ substLeftInputEnv ΓΔ pΓΔ pΓ
+      = Γ₁ ∘ Δ
+    ⟫.
+Proof. induction peΓΔ; crush. Qed.
+Hint Resolve substLeftInput.
 
-Lemma substPart_inl_partenv {p Γ Γ₁ Γ₂} (pe: ⟪ p ⊢ Γ = Γ₁ ∘ Γ₂ ⟫) :
-  ∀ i j Δ,
-    isLeftOrRight p i = inl j →
-    ⟪ substPart p i (dom Δ) ⊢ insertEnv Δ Γ i = insertEnv Δ Γ₁ j ∘ Γ₂ ⟫.
-Proof. induction pe; crush. Qed.
+Fixpoint substRightInputEnv (ΓΔ: Env) (pΓΔ pΓ: Part) : Env :=
+  match ΓΔ , pΓΔ , pΓ with
+    | ε      , _          , _         => ε
+    | _      , pnil       , _         => ε
+    | ΓΔ ▻ a , pleft pΓΔ  , pnil      => ε
+    | ΓΔ ▻ a , pleft pΓΔ  , pleft pΓ  => substRightInputEnv ΓΔ pΓΔ pΓ
+    | ΓΔ ▻ a , pleft pΓΔ  , pright pΓ => substRightInputEnv ΓΔ pΓΔ pΓ ▻ a
+    | ΓΔ ▻ a , pright pΓΔ , pΓ        => substRightInputEnv ΓΔ pΓΔ pΓ ▻ a
+  end.
 
-Lemma substPart_inr_partenv {p Γ Γ₁ Γ₂} (pe: ⟪ p ⊢ Γ = Γ₁ ∘ Γ₂ ⟫) :
-  ∀ i j Δ,
-    isLeftOrRight p i = inr j →
-    ⟪ substPart p i (dom Δ) ⊢ insertEnv Δ Γ i = Γ₁ ∘ insertEnv Δ Γ₂ j ⟫.
-Proof. induction pe; crush. Qed.
+Fixpoint substRightInputPart (pΓΔ pΓ: Part) : Part :=
+  match pΓΔ , pΓ with
+    | pnil       , _         => pnil
+    | pleft _    , pnil      => pnil
+    | pleft pΓΔ  , pleft pΓ  => substRightInputPart pΓΔ pΓ
+    | pleft pΓΔ  , pright pΓ => pleft (substRightInputPart pΓΔ pΓ)
+    | pright pΓΔ , pΓ        => pright (substRightInputPart pΓΔ pΓ)
+  end.
 
-(* Substitute index i in t by term s which has δ free variables. *)
-Fixpoint subst (i: Ix) (s: Tm) (δ: Dom) (t: Tm) : Tm :=
+Lemma substRightInput {pΓΔ ΓΔ Γ Δ} (peΓΔ : ⟪ pΓΔ ⊢ ΓΔ = Γ ∘ Δ ⟫) :
+  ∀ {pΓ Γ₁ Γ₂},
+    ⟪ pΓ ⊢ Γ = Γ₁ ∘ Γ₂ ⟫ →
+    ⟪ substRightInputPart pΓΔ pΓ ⊢ substRightInputEnv ΓΔ pΓΔ pΓ = Γ₂ ∘ Δ ⟫.
+Proof. induction peΓΔ; crush. Qed.
+Hint Resolve substRightInput.
+
+Fixpoint substLeftResultPart' (pΓΔ pΓ: Part) : Part :=
+  match pΓΔ , pΓ with
+    | pnil         , _         => pnil
+    | pleft _      , pnil      => pnil
+    | pleft pΓΔ    , pleft pΓ  => pleft (substLeftResultPart' pΓΔ pΓ)
+    | pleft pΓΔ    , pright pΓ => pright (substLeftResultPart' pΓΔ pΓ)
+    | pright pΓΔ   , pΓ        => pleft (substLeftResultPart' pΓΔ pΓ)
+  end.
+
+Lemma substLeftResult' {pΓΔ ΓΔ Γ Δ} (peΓΔ : ⟪ pΓΔ ⊢ ΓΔ = Γ ∘ Δ ⟫) :
+  ∀ {pΓ Γ₁ Γ₂},
+    ⟪ pΓ ⊢ Γ = Γ₁ ∘ Γ₂ ⟫ →
+    ⟪ substLeftResultPart' pΓΔ pΓ ⊢ ΓΔ = substLeftInputEnv ΓΔ pΓΔ pΓ ∘ Γ₂ ⟫.
+Proof. induction peΓΔ; crush. Qed.
+Hint Resolve substLeftResult'.
+
+Fixpoint substRightResultPart' (pΓΔ pΓ: Part) : Part :=
+  match pΓΔ , pΓ with
+    | pnil         , _         => pnil
+    | pleft _      , pnil      => pnil
+    | pleft pΓΔ    , pleft pΓ  => pleft (substRightResultPart' pΓΔ pΓ)
+    | pleft pΓΔ    , pright pΓ => pright (substRightResultPart' pΓΔ pΓ)
+    | pright pΓΔ   , pΓ        => pright (substRightResultPart' pΓΔ pΓ)
+  end.
+
+Lemma substRightResult' {pΓΔ ΓΔ Γ Δ} (peΓΔ : ⟪ pΓΔ ⊢ ΓΔ = Γ ∘ Δ ⟫) :
+  ∀ {pΓ Γ₁ Γ₂},
+    ⟪ pΓ ⊢ Γ = Γ₁ ∘ Γ₂ ⟫ →
+    ⟪ substRightResultPart' pΓΔ pΓ ⊢ ΓΔ = Γ₁ ∘ substRightInputEnv ΓΔ pΓΔ pΓ ⟫.
+Proof. induction peΓΔ; crush. Qed.
+Hint Resolve substRightResult'.
+
+Fixpoint substResultEnv (ΓΔ: Env) (pΓΔ: Part) (i: Ix) : Env :=
+  match ΓΔ , pΓΔ , i with
+    | ε      , _          , _   => ε
+    | _      , pnil       , _   => ε
+    | ΓΔ ▻ a , pleft pΓΔ  , O   => ΓΔ
+    | ΓΔ ▻ a , pleft pΓΔ  , S i => substResultEnv ΓΔ pΓΔ i ▻ a
+    | ΓΔ ▻ a , pright pΓΔ , i   => substResultEnv ΓΔ pΓΔ i ▻ a
+  end.
+
+Fixpoint substLeftResultPart (pΓΔ pΓ: Part) (j: Ix) : Part :=
+  match pΓΔ , pΓ , j with
+    | pnil       , _          , _   => pnil
+    | pleft _    , pnil       , _   => pnil
+    | pleft pΓΔ  , pleft pΓ   , O   => substLeftResultPart' pΓΔ pΓ
+    | pleft pΓΔ  , pleft pΓ   , S j => pleft (substLeftResultPart pΓΔ pΓ j)
+    | pleft pΓΔ  , pright pΓ  , j   => pright (substLeftResultPart pΓΔ pΓ j)
+    | pright pΓΔ , pΓ         , j   => pleft (substLeftResultPart pΓΔ pΓ j)
+  end.
+
+Lemma substLeftResult {pΓΔ ΓΔ Γ Δ} (peΓΔ : ⟪ pΓΔ ⊢ ΓΔ = Γ ∘ Δ ⟫) :
+  ∀ {j b pΓ Γ₁ Γ₂},
+    ⟪ j : b ∈ Γ₁ ⟫ →
+    ⟪ pΓ ⊢ Γ = Γ₁ ∘ Γ₂ ⟫ →
+    ⟪ substLeftResultPart pΓΔ pΓ j ⊢ substResultEnv ΓΔ pΓΔ (fromLeft pΓ j) =
+      substResultEnv (substLeftInputEnv ΓΔ pΓΔ pΓ) (substLeftInputPart pΓΔ pΓ) j ∘ Γ₂
+    ⟫.
+Proof. induction peΓΔ; crush. Qed.
+Hint Resolve substLeftResult.
+
+Fixpoint substRightResultPart (pΓΔ pΓ: Part) (j: Ix) : Part :=
+  match pΓΔ , pΓ , j with
+    | pnil       , _          , _   => pnil
+    | pleft _    , pnil       , _   => pnil
+    | pleft pΓΔ  , pleft pΓ   , j   => pleft (substRightResultPart pΓΔ pΓ j)
+    | pleft pΓΔ  , pright pΓ  , O   => substRightResultPart' pΓΔ pΓ
+    | pleft pΓΔ  , pright pΓ  , S j => pright (substRightResultPart pΓΔ pΓ j)
+    | pright pΓΔ , pΓ         , j   => pright (substRightResultPart pΓΔ pΓ j)
+  end.
+
+Lemma substRightResult {pΓΔ ΓΔ Γ Δ} (peΓΔ : ⟪ pΓΔ ⊢ ΓΔ = Γ ∘ Δ ⟫) :
+  ∀ {j b pΓ Γ₁ Γ₂},
+    ⟪ j : b ∈ Γ₂ ⟫ →
+    ⟪ pΓ ⊢ Γ = Γ₁ ∘ Γ₂ ⟫ →
+    ⟪ substRightResultPart pΓΔ pΓ j ⊢ substResultEnv ΓΔ pΓΔ (fromRight pΓ j) =
+      Γ₁ ∘ substResultEnv (substRightInputEnv ΓΔ pΓΔ pΓ) (substRightInputPart pΓΔ pΓ) j
+    ⟫.
+Proof. induction peΓΔ; crush. Qed.
+Hint Resolve substRightResult.
+
+Lemma substResultEnv_singleton {pΓΔ ΓΔ Δ b} (peΓΔ : ⟪ pΓΔ ⊢ ΓΔ = ε ▻ b ∘ Δ ⟫) :
+  Δ = substResultEnv ΓΔ pΓΔ O.
+Proof. depind peΓΔ; crush. Qed.
+
+Fixpoint substTm (i: Ix) (pΓΔ: Part) (s t: Tm) : Tm :=
   match t with
     | var _       => s
-    | abs b t     => abs b (subst (S i) s δ t)
-    | app p t₁ t₂ =>
-      match isLeftOrRight p i with
-        | inl i' => app (substPart p i δ) (subst i' s δ t₁) t₂
-        | inr i' => app (substPart p i δ) t₁ (subst i' s δ t₂)
+    | abs a t     => abs a (substTm (S i) (pleft pΓΔ) s t)
+    | app pΓ t₁ t₂ =>
+      match isLeftOrRight pΓ i with
+        | inl j => (* j ∈ γ₁ *)
+          app (substLeftResultPart pΓΔ pΓ j) (substTm j (substLeftInputPart pΓΔ pΓ) s t₁) t₂
+        | inr j => (* j ∈ γ₂ *)
+          app (substRightResultPart pΓΔ pΓ j) t₁ (substTm j (substRightInputPart pΓΔ pΓ) s t₂)
       end
   end.
 
-Lemma subst_wsTm {γ t s δ} (ws: ⟨δ ⊢ s⟩) (wt: ⟨γ ⊢ t⟩) :
-  ∀ i, ⟨i ∈ γ⟩ → ⟨insertDom δ γ i ⊢ subst i s δ t⟩.
+Lemma substWtTm {Δ s b Γ t a} (ws: ⟪ Δ ⊢ s : b⟫) (wt: ⟪ Γ ⊢ t : a ⟫) :
+  ∀ {i pΓΔ ΓΔ} (wi : ⟪ i : b ∈ Γ⟫) (peΓΔ : ⟪ pΓΔ ⊢ ΓΔ = Γ ∘ Δ ⟫),
+    ⟪ substResultEnv ΓΔ pΓΔ i ⊢ substTm i pΓΔ s t : a ⟫.
 Proof.
-  induction wt; crush.
+  induction wt; simpl; intros.
+  - apply substResultEnv_singleton in peΓΔ; crush.
   - constructor.
-    apply (IHwt (S i)); crush.
-  - econstructor; eauto.
-    eapply substPart_inl_partdom; eauto.
-    apply isLeftOrRight_inl_sound in Heqs0; crush.
-  - econstructor; eauto.
-    eapply substPart_inr_partdom; eauto.
-    apply isLeftOrRight_inr_sound in Heqs0; crush.
+    apply (IHwt (S i) (pleft pΓΔ) (ΓΔ ▻ a)); crush.
+  - crush; econstructor; crush.
 Qed.
 
-Lemma subst_wtTm {Γ Δ s b t a} (ws: ⟪ Δ ⊢ s : b ⟫) (wt: ⟪ Γ ⊢ t : a ⟫) :
-  ∀ i, ⟪ i : b ∈ Γ ⟫ → ⟪ insertEnv Δ Γ i ⊢ subst i s (dom Δ) t : a ⟫.
+
+Lemma subst0_wtTm {pΓΔ ΓΔ Γ Δ s b t a}
+  (ws: ⟪ Δ ⊢ s : b ⟫) (wt: ⟪ Γ ▻ b ⊢ t : a ⟫)
+  (peΓΔ: ⟪ pΓΔ ⊢ ΓΔ = Γ ∘ Δ ⟫) :
+  ⟪ ΓΔ ⊢ substTm 0 (pleft pΓΔ) s t : a ⟫.
+Proof. apply (substWtTm ws wt inEnvO (PELeft peΓΔ)). Qed.
+
+Inductive Substs : Set :=
+  | SNil
+  | SSnoc (σ: Substs) (p: Part) (s: Tm).
+
+Fixpoint substsTm (σ: Substs) (t: Tm) : Tm :=
+  match σ with
+    | SNil          => t
+    | SSnoc σ pΓΔ s => substsTm σ (substTm 0 (pleft pΓΔ) s t)
+  end.
+
+Inductive WtSubsts : Substs → Env → Env → Prop :=
+  | WtSNil {Γ} :
+      WtSubsts SNil Γ Γ
+  | WtSSnoc {σ Σ ΓΔ Γ Δ pΓΔ s b} :
+      WtSubsts σ ΓΔ Σ →
+      ⟪ pΓΔ ⊢ ΓΔ = Γ ∘ Δ ⟫ →
+      ⟪ Δ ⊢ s : b ⟫ →
+      WtSubsts (SSnoc σ pΓΔ s) (Γ ▻ b) Σ.
+
+Lemma substsWtTm {σ Γ Δ} (wσ: WtSubsts σ Γ Δ) :
+  ∀ {t a}, ⟪ Γ ⊢ t : a ⟫ → ⟪ Δ ⊢ substsTm σ t : a ⟫.
 Proof.
-  induction wt; crush.
-  - inversion H; subst.
-    + rewrite ecat_left_empty; auto.
-    + inversion H4.
-  - constructor.
-    apply (IHwt (S i)); crush.
-    constructor.
-    eauto.
-  - econstructor; crush.
-    eapply substPart_inl_partenv; crush.
-    eapply IHwt1.
-    apply (wtix_isLeftOrRight_inl H H0 Heqs0).
-  - econstructor; crush.
-    eapply substPart_inr_partenv; crush.
-    eapply IHwt2; crush.
-    apply (wtix_isLeftOrRight_inr H H0 Heqs0).
+  induction wσ; simpl; intros.
+  - eauto.
+  - eapply IHwσ.
+    eapply subst0_wtTm; eauto.
 Qed.
 
-Lemma subst_wtTm_closed {s b t a} (ws: ⟪ ε ⊢ s : b ⟫) (wt: ⟪ [b] ⊢ t : a ⟫) :
-  ⟪ ε ⊢ subst 0 s 0 t : a ⟫.
-Proof. apply (subst_wtTm ws wt 0). constructor. Qed.
+(*  Γ,Δ₂,Δ₁   Γ,Δ₂,Δ₁              *)
+(*    ⇓ σ₁                         *)
+(*  Γ,Δ₂        ⇓ σ₁ >>= σ₂        *)
+(*    ⇓ σ₂                         *)
+(*  Γ         Γ                    *)
+Fixpoint substsComp (σ₁ σ₂: Substs) : Substs :=
+  match σ₁ with
+    | SNil         => σ₂
+    | SSnoc σ₁ p s => SSnoc (substsComp σ₁ σ₂) p s
+  end.
+Notation "σ₁ >>= σ₂" := (substsComp σ₁ σ₂) (at level 42, left associativity).
+
+Lemma wtsubsts_comp {σ₁ Γ Δ} (wσ₁: WtSubsts σ₁ Γ Δ) :
+  ∀ σ₂ Σ,
+    WtSubsts σ₂ Δ Σ →
+    WtSubsts (σ₁ >>= σ₂) Γ Σ.
+Proof.
+  induction wσ₁; simpl; try econstructor; eauto.
+Qed.
+
 
 Fixpoint Value (t: Tm) : Prop :=
   match t with
@@ -462,12 +669,15 @@ Fixpoint Value (t: Tm) : Prop :=
 
 Reserved Notation "t₁ --> t₂" (at level 40).
 Inductive red : Tm → Tm → Prop :=
-  | red_beta {a t₁ t₂} :
-      app pnil (abs a t₁) t₂ --> subst 0 t₂ 0 t₁
-  | red_app₁ {t₁ t₁' t₂} :
-      t₁ --> t₁' → app pnil t₁ t₂ --> app pnil t₁' t₂
-  | red_app₂ {t₁ t₂ t₂'} :
-      Value t₁ → t₂ --> t₂' → app pnil t₁ t₂ --> app pnil t₁ t₂'
+  | red_abs {a t t'} :
+      t --> t' →
+      abs a t --> abs a t'
+  | red_app₁ {p t₁ t₁' t₂} :
+      t₁ --> t₁' → app p t₁ t₂ --> app p t₁' t₂
+  | red_app₂ {p t₁ t₂ t₂'} :
+      t₂ --> t₂' → app p t₁ t₂ --> app p t₁ t₂'
+  | red_beta {p a t₁ t₂} :
+      app p (abs a t₁) t₂ --> substTm 0 (pleft p) t₂ t₁
 where "t₁ --> t₂" := (red t₁ t₂).
 
 Lemma can_form_tarr {Γ t a b}
@@ -485,18 +695,148 @@ Proof with try (subst; eauto using red).
   destruct (can_form_tarr v1 wt1)...
 Qed.
 
-Lemma preservation {t a} (wt: ⟪ ε ⊢ t : a ⟫) :
-  ∀ {t'}, t --> t' → ⟪ ε ⊢ t' : a ⟫.
+Lemma preservation {Γ t a} (wt: ⟪ Γ ⊢ t : a ⟫) :
+  ∀ {t'}, t --> t' → ⟪ Γ ⊢ t' : a ⟫.
 Proof.
-  depind wt.
-  - inversion 1; crush.
-  - inversion H; subst.
-    specialize (IHwt1 eq_refl).
-    specialize (IHwt2 eq_refl).
-    clear H.
-    inversion 1; subst.
+  induction wt.
+  - inversion 1.
+  - intros t' r; inversion r; subst.
+    econstructor; eauto.
+  - intros t' r; inversion r; subst.
+    + econstructor; eauto.
+    + econstructor; eauto.
     + inversion wt1; subst.
-      eapply subst_wtTm_closed; eauto.
-    + econstructor; eauto.
-    + econstructor; eauto.
+      eapply subst0_wtTm; eauto.
+Qed.
+
+Lemma red_subst i p s :
+  ∀ {t t'}, t --> t' → substTm i p s t --> substTm i p s t'.
+Proof.
+Admitted.
+
+Inductive SN (t : Tm) : Prop :=
+  | SNi : (∀ t', t --> t' → SN t') → SN t.
+
+Lemma SNd {t} (sn_t: SN t) : ∀ t', t --> t' → SN t'.
+Proof. destruct sn_t; auto. Qed.
+
+Lemma SNappl {t1} p t2 (sn: SN (app p t1 t2)) : SN t1.
+Proof.
+  depind sn; constructor; intros; subst.
+  eapply H0; eauto using red.
+Qed.
+
+Lemma SNvar {t} p n (sn: SN (substTm 0 p (var n) t)) : SN t.
+Proof. depind sn; constructor; eauto using red_subst. Qed.
+
+Definition Cand := Tm → Prop.
+Definition Neutral : Cand :=
+  fun t => match t with
+             | abs _ _ => False
+             | _       => True
+           end.
+
+(* Definition of reducibility candidates. *)
+Record CR (P: Cand) :=
+  { cr_sn : ∀ t, P t → SN t;
+    cr_cl : ∀ t, P t → ∀ t', t --> t' → P t';
+    cr_nt : ∀ t, Neutral t → (∀ t', t --> t' → P t') → P t
+  }.
+Arguments cr_sn [_] _ [_] _.
+Arguments cr_cl [_] _ [_] _ [_] _.
+Arguments cr_nt [_] _ [_] _ _.
+
+Lemma CR_var {P:Cand} (crP : CR P) : ∀ n, P (var n).
+Proof.
+  intros; apply cr_nt; simpl; auto; intros.
+  inversion H.
+Qed.
+
+Lemma CR_SN : CR SN.
+Proof. constructor; eauto using SNd, SNi. Qed.
+
+Definition ARR (P R: Cand) : Cand :=
+  fun (t1: Tm) => ∀ p t2, P t2 → R (app p t1 t2).
+
+Lemma CR_ARR {P R} {CR_P: CR P} {CR_R: CR R} : CR (ARR P R).
+Proof with simpl; eauto using red.
+  constructor.
+  - intros t ARR_t.
+    (* This is soo ugly. *)
+    eapply (SNappl pnil (var 0)).
+    eapply (cr_sn CR_R), ARR_t, CR_var...
+  - intros t ARR_t t' r p s P_s.
+    eapply (cr_cl CR_R)...
+  - intros t neutral_t Hyp p t' P_t'.
+    apply (cr_nt CR_R)...
+    generalize (cr_sn CR_P P_t').
+    induction 1 as [t']; intros t'' r.
+    inversion r; subst.
+    + eapply Hyp...
+    + eapply cr_nt...
+      eapply H0...
+      eapply cr_cl...
+    + destruct neutral_t.
+Qed.
+
+Lemma Lam_Sound {P R} (crP: CR P) (crR: CR R) :
+  ∀ T M, (∀ p N, P N → R (substTm 0 p N M)) →
+    ARR P R (abs T M).
+Proof.
+  intros T M H.
+  assert (SN_M : SN M) by eauto using (SNvar pnil 0), (cr_sn crR), (CR_var crP).
+  revert H.
+  induction SN_M; intros Hyp p1 L1 ?.
+  assert (SN_L1: SN L1) by eauto using (cr_sn crP).
+  induction SN_L1.
+  apply (cr_nt crR); simpl; auto.
+  intros ? r.
+  depind r; eauto.
+  * dependent destruction r; eauto.
+    unfold ARR in *; eauto using (cr_cl crR), red_subst.
+  * eauto using (cr_cl crP).
+Qed.
+
+(* Type interpretation *)
+Fixpoint Int (T: Ty) : Cand :=
+  match T with
+    | tbase      => SN
+    | tarr T1 T2 => ARR (Int T1) (Int T2)
+  end.
+
+Lemma CR_Int (T: Ty) : CR (Int T).
+Proof.
+  induction T; eauto using CR_SN, CR_ARR.
+Qed.
+
+(* Definition IntEnv Γ (σ: Substs) : Prop := *)
+(*   ∀ x T, lookup_evar Γ x T → Int T (substsTm σ (var x)). *)
+
+(* Lemma Int_sound {Γ M T} (wt: Typing Γ M T) : *)
+(*   ∀ σ, IntEnv Γ σ → Int T (M[σ]). *)
+(* Proof. *)
+(*   induction wt; intros σ IntEnv_Γ; simpl; auto using SNtt. *)
+(*   - apply Lam_Sound; simpl; intros; eauto using CR_Int. *)
+(*     rewrite sub_inst_comp. *)
+(*     apply IHwt; simpl. *)
+(*     unfold IntEnv; intros. *)
+(*     dependent destruction H0; simpl. *)
+(*     + rewrite sub_up1_def; simpl. *)
+(*       rewrite sub_comp_snoc; simpl. *)
+(*       auto. *)
+(*     + rewrite sub_up1_def; simpl. *)
+(*       rewrite sub_comp_snoc; simpl. *)
+(*       rewrite sub_comp_assoc; simpl. *)
+(*       rewrite sub_comp_id_right; simpl. *)
+(*       auto. *)
+(*   - simpl in *; unfold ARR in *; auto. *)
+(* Qed. *)
+
+Lemma Int_sound_id {Γ M T} (wt: ⟪ Γ ⊢ M : T ⟫) : Int T M.
+Proof.
+Admitted.
+
+Theorem strong_normalization {Γ t T} (wt: ⟪ Γ ⊢ t : T ⟫) : SN t.
+Proof.
+  eauto using (cr_sn (CR_Int T)), Int_sound_id.
 Qed.
